fix assertion failure in InsertModel

lib/Buckets/BucketsLib.i.dfy
@@ -47,9 +47,16 @@ module BucketsLib {
   {
     function as_map() : BucketMap
     requires |this.keys| == |this.msgs|
+    ensures WFBucket(this) ==> WFBucketMap(as_map())
     {
+      value_sets_le(keys, msgs);
       map_of_seqs(keys, msgs)
     }
+  }
+
+  predicate WFBucketMap(bucket: BucketMap)
+  {
+    forall message: Message :: message in bucket.Values ==> message != IdentityMessage()
   }
 
   type BucketList = seq<Bucket>
@@ -183,13 +190,35 @@ module BucketsLib {
   ensures PreWFBucket(b)
   ensures IsStrictlySorted(b.keys)
   ensures b.as_map() == m
-  {
+  ensures WFBucketMap(m) ==> WFBucket(b)
+  {  
     IsStrictlySorted_seqs_of_map(m);
     map_of_seqs_of_seqs_of_map(m);
     var sp := seqs_of_map(m);
     var b := Bucket(sp.keys, sp.msgs);
     assert b.as_map() == map_of_seqs(b.keys, b.msgs);
+    test(m, sp, b);
     b
+  }
+
+  lemma test(m: map<Key, Message>, sp: SeqPair, b: Bucket)
+  requires sp == seqs_of_map(m);
+  requires b == Bucket(sp.keys, sp.msgs);
+  ensures WFBucketMap(m) ==> WFBucket(b)
+  {
+    if WFBucketMap(m) {
+      assert Set(b.msgs) == m.Values by {
+        seqs_of_map_preserves_values(m, sp);
+      }
+      assert forall i : int :: 0 <= i < |b.msgs| ==> b.msgs[i] != IdentityMessage()
+      by {
+        forall i | 0 <= i < |b.msgs|
+          ensures b.msgs[i] != IdentityMessage()
+        {
+          assert b.msgs[i] in m.Values;
+        }
+      }
+    }
   }
 
   function BucketInsert(bucket: Bucket, key: Key, msg: Message) : Bucket
